Current status: new definition of Instr.t, but has to be changed to remove reductions of match ... with eq_refl => ...

typed-assembly/StaticCode.v
@@ -18,54 +18,134 @@ Fixpoint valid_nth A (l : list A) (n : nat) (H : n < length l) : A.
     now apply lt_S_n.
 Defined.
 
+(*Module Ip.
+  Definition t : Set := nat.
+  
+  Definition tl (size : nat) : Set := {ip : nat | ip < size}.
+  
+  (*Definition is_valid (ip : t) (size : nat) :=
+    match ip with
+    | None => True
+    | Some ip => ip < size
+    end.*)
+End Ip.*)
+
 Module Instr.
-  Definition t (S : Set) (L : S -> Type)
-    (lt : (nat * sigT L) -> (nat * sigT L) -> Prop) (Hwf : well_founded lt)
-    (size : nat) : Type :=
-    forall s ip, {s'_next_ip : S * nat &
-      let (s', next_ip) := s'_next_ip in
-      forall (l : L s), Datatypes.S ip <= size -> (next_ip <= size) * {l' : L s' |
-      lt (next_ip, existT _ _ l') (Datatypes.S ip, existT _ _ l) }}.
+  Open Local Scope type.
+  
+  Definition lt_type (S : Set) (L : nat -> S -> Type) :=
+    {ip : nat & {s : S & L ip s}} -> {ip : nat & {s : S & L ip s}} -> Prop.
+  
+  Definition t (S : Set) (L : nat -> S -> Type) (lt : lt_type L) (Hwf : well_founded lt)
+    : Type :=
+    {ip : nat & forall s, {ip' : nat & {s' : S &
+      forall (l : L ip s), {l' : L ip' s' |
+        lt (existT _ _ (existT _ _ l')) (existT _ _ (existT _ _ l)) }}}}.
   
   (** Simple eval of just one instruction (for tests) *)
-  Definition eval (S : Set) (L : S -> Type)
-    (lt : (nat * sigT L) -> (nat * sigT L) -> Prop) (Hwf : well_founded lt)
-    (size : nat) (i : t Hwf size)
-    (ip : nat) (s : S) (l : L s) (Hip_valid : Datatypes.S ip <= size)
-    : {next_ip : nat | next_ip <= size} * {s' : S & L s'}.
-    destruct (i s ip) as ((s', next_ip), fl).
-    destruct (fl l Hip_valid) as (Hnext_ip_valid, (l', _)).
-    exact (exist _ next_ip Hnext_ip_valid, existT _ s' l').
+  Definition eval (S : Set) (L : nat -> S -> Type) (lt : lt_type L) (Hwf : well_founded lt)
+    (i : t Hwf) (s : S) (l : L (projT1 i) s)
+    : {ip' : nat & {s' : S & L ip' s'}}.
+    destruct i as (ip, f); simpl in l.
+    destruct (f s) as (ip', (s', fl)).
+    destruct (fl l) as (l', _).
+    now exists ip'; exists s'.
   Defined.
 End Instr.
 
 Module Program.
-  Definition t (S : Set) (L : S -> Type)
-    (lt : (nat * sigT L) -> (nat * sigT L) -> Prop) (Hwf : well_founded lt)
-    (size : nat) : Type :=
-    list (Instr.t Hwf size).
+  Definition t (S : Set) (L : nat -> S -> Type) (lt : Instr.lt_type L) (Hwf : well_founded lt)
+    : Type :=
+    list (Instr.t Hwf).
   
-  (** The instruction pointer [ip] is decrementing during the evaluation, down to zero. *)
-  Definition eval (S : Set) (L : S -> Type)
-    (lt_L : (nat * sigT L) -> (nat * sigT L) -> Prop) (Hwf : well_founded lt_L)
-    (size : nat) (p : t Hwf size) (Hp_valid : size = length p)
-    : forall (input : nat * {s : S & L s}) (Hip_valid : fst input <= size),
-      {s : S & L s}.
-    refine (well_founded_induction_type Hwf _ _).
-    intros input eval Hip_valid.
-    destruct input as (ip, (s, l)).
-    destruct ip as [|ip].
-      (* [ip] is null, the program is terminated. *)
-      exact (existT _ _ l).
+  (*Definition is_valid (S : Set) (L : nat -> S -> Type)
+    (lt : {ip : nat & {s : S & L ip s}} -> {ip : nat & {s : S & L ip s}} -> Prop) (Hwf : well_founded lt)
+    (p : t L Hwf) : Prop :=
+    let fix aux p (ip : nat) : Prop :=
+      match p with
+      | nil => True
+      | existT _ ip' _ :: p => ip' = ip /\ aux p (Datatypes.S ip)
+      end in
+    aux p 0.
+  
+  Lemma is_valid_nth (S : Set) (L : nat -> S -> Type)
+    (lt : {ip : nat & {s : S & L ip s}} -> {ip : nat & {s : S & L ip s}} -> Prop) (Hwf : well_founded lt)
+    (p : t L Hwf) (H : is_valid p)
+    : forall (ip : nat) (Hip : ip < length p), projT1 (valid_nth p Hip) = ip.
+    induction p; intros ip Hip; simpl in H.
+      admit.
       
-      (* [ip] is not null, one instruction is executed. *)
-      refine (let i := valid_nth p (n := ip) _ in _).
-        rewrite Hp_valid in Hip_valid.
-        apply lt_S_n.
-        now apply le_lt_n_Sm.
-      destruct (i s ip) as ((s', next_ip), fl).
-      destruct (fl l Hip_valid) as (Hnext_ip_valid, (l', Hl'_lt_l)).
-      exact (eval (next_ip, existT _ _ l') Hl'_lt_l Hnext_ip_valid).
+      destruct ip as [|ip]; simpl.
+        unfold is_valid in H.
+        destruct a as (ip', f); simpl in *.
+        tauto.
+        
+        unfold is_valid in H.
+        simpl.
+        unfold is_valid in H; simpl in H.
+  Admitted.*)
+  
+  Definition is_valid (S : Set) (L : nat -> S -> Type) (lt : Instr.lt_type L) (Hwf : well_founded lt)
+    (p : t Hwf) : Prop :=
+    forall (ip : nat) (H : ip < length p), projT1 (valid_nth p H) = ip.
+  
+  Definition is_valid_aux (S : Set) (L : nat -> S -> Type) (lt : Instr.lt_type L) (Hwf : well_founded lt)
+    (p : t Hwf) (ip0 : nat) : Prop :=
+    forall (ip : nat) (H : ip < length p), projT1 (valid_nth p H) = ip0 + ip.
+  
+  (** All sub-proofs are made transparent for reduction. *)
+  Fixpoint decide_is_valid_aux (S : Set) (L : nat -> S -> Type) (lt : Instr.lt_type L) (Hwf : well_founded lt)
+    (p : t Hwf) (ip0 : nat) : option (is_valid_aux p ip0).
+    destruct p as [|i p].
+      refine (Some _); unfold is_valid; intros ip H.
+      unfold Peano.lt in H.
+      simpl in H.
+      inversion H.
+      
+      destruct i as (ip', f).
+      destruct (eq_nat_dec ip0 ip') as [Hip0_ip' | _]; [| exact None].
+      destruct (decide_is_valid_aux _ _ _ _ p (1 + ip0)) as [Hp |]; [| exact None].
+      refine (Some _); unfold is_valid; intros ip H.
+      destruct ip as [|ip]; simpl in *.
+        now rewrite Hip0_ip'.
+        
+        unfold is_valid_aux in Hp.
+        assert (Haux : forall n m, n + Datatypes.S m = Datatypes.S n + m).
+          intros n m; induction n; trivial.
+          simpl; now rewrite IHn.
+        rewrite Haux.
+        apply Hp.
+  Defined.
+  
+  Definition decide_is_valid (S : Set) (L : nat -> S -> Type) (lt : Instr.lt_type L) (Hwf : well_founded lt)
+    (p : t Hwf) : option (is_valid p) :=
+    decide_is_valid_aux p 0.
+  
+  Definition reflexive_is_valid (S : Set) (L : nat -> S -> Type) (lt : Instr.lt_type L) (Hwf : well_founded lt)
+    (p : t Hwf) (H : (if decide_is_valid p then true else false) = true) : is_valid p.
+    now destruct (decide_is_valid p) as [Hvalid |].
+  Defined.
+  
+  Definition eval (S : Set) (L : nat -> S -> Type) (lt : Instr.lt_type L) (Hwf : well_founded lt)
+    (p : t Hwf) (Hp_valid : is_valid p) (s : S) (l : L 0 s)
+    : {ip' : nat & {s' : S & L ip' s'}}.
+    refine (let aux : {ip' : nat & {s' : S & L ip' s'}} -> _ := _ in
+      aux (existT _ _ (existT _ _ l))).
+    clear s l.
+    refine (well_founded_induction_type Hwf _ _).
+    intros input eval.
+    destruct input as (ip, (s, l)).
+    destruct (le_lt_dec (length p) ip) as [Hge | Hlt].
+      (* ip >= length p, the program is terminated. *)
+      exact (existT _ _ (existT _ _ l)).
+      
+      (* ip < length p, one instruction is executed. *)
+      assert (Hip'_ip := Hp_valid ip Hlt).
+      destruct (valid_nth p Hlt) as (ip', f); simpl in Hip'_ip.
+      rewrite Hip'_ip in f; clear Hip'_ip ip'.
+      destruct (f s) as (ip', (s', fl)).
+      destruct (fl l) as (l', Hl'_lt_l).
+      exact (eval (existT _ _ (existT _ _ l')) Hl'_lt_l).
   Defined.
 End Program.
 
@@ -74,32 +154,46 @@ Module Test1.
   
   Definition S := nat.
   
-  Definition L (n : S) : Prop :=
+  Definition L (ip : nat) (n : S) : Prop :=
     3 <= n.
   
-  Definition lt (x y : nat * sigT L) : Prop :=
-    fst x < fst y.
+  Definition size := 2.
+  
+  Definition f_lt T (x : {ip : nat & T ip}) : nat :=
+    if leb size (projT1 x) then
+      0
+    else
+      (projT1 x) + 1.
+  
+  Definition lt : Instr.lt_type L := fun x y =>
+    f_lt _ x < f_lt _ y.
   
   (** Has to be transparent to reduce the well-founded recursion. *)
   Lemma lt_wf : well_founded lt.
     apply well_founded_ltof.
   Defined.
   
-  Definition size := 2.
-  
   (** A program where the state is a single natural number, and the logical world
       a proof that it is greater or equal to three. *)
-  Definition progr : Program.t lt_wf size.
+  Definition progr : Program.t lt_wf.
     refine [
-      (fun n ip => existT _ (n + 1, ip) _);
-      (fun _ ip => existT _ (12, ip) _)];
-      unfold S, L, lt; intros l Hip_valid;
-      (split; [now apply le_Sn_le |]);
-      [assert (H : L (n + 1)) | assert (H : 3 <= 12)]; unfold L; auto with arith;
-      apply exist with (x := H); auto.
+      existT _ 0 (fun n => existT _ size (existT _ (n + 1) _)); (* n := n + 1 *)
+      existT _ 1 (fun n => existT _ 0 (existT _ 12 _))]; (* n := 12 *)
+      unfold L, lt, f_lt; intro l;
+      [assert (H : 3 <= n + 1) | assert (H : 3 <= 12)]; unfold L; auto with arith;
+      exists H; auto.
   Defined.
   
-  Definition input : nat * {s : S & L s}.
+  Definition progr_is_valid : Program.is_valid progr :=
+    Program.reflexive_is_valid progr eq_refl.
+  
+  Definition progr_is_valid' : Program.is_valid progr.
+  Admitted.
+  
+  Compute projT1 (Program.eval progr_is_valid 23 (leb_complete 3 23 eq_refl)).
+  Compute projT1 (Program.eval progr_is_valid' 23 (leb_complete 3 23 eq_refl)).
+  
+  (*Definition input : nat * {s : S & L s}.
     refine (2, existT _ 23 _).
     unfold L; auto with *.
   Defined.
@@ -130,42 +224,92 @@ Module Test1.
   Defined.
   
   Compute projT1 (Program.eval progr_small eq_refl
-    (1, existT _ 23 (leb_complete 3 23 eq_refl)) (leb_complete 1 1 eq_refl)).
-  
-  Compute projT1 (Program.eval progr eq_refl input input_is_valid).
+    (1, existT _ 23 (leb_complete 3 23 eq_refl)) (leb_complete 1 1 eq_refl)).*)
 End Test1.
+
+(** A language with arithmetic expressions and assertions *)
+Module Arith.
+  Require Import ZArith.
+  
+  Local Open Scope Z_scope.
+  
+(*   Definition subZ P := {z : Z | P z}. *)
+  
+  Inductive t : (Z -> Prop) -> Type :=
+  | const : forall (P : Z -> Prop) z, P z -> t P
+  | uminus : forall (P1 P : Z -> Prop), t P1 ->
+    (forall z, P1 z -> P (- z)) -> t P
+  | plus : forall (P1 P2 P : Z -> Prop), t P1 -> t P2 ->
+    (forall z1 z2, P1 z1 -> P2 z2 -> P (z1 + z2)) -> t P
+  | times : forall (P1 P2 P : Z -> Prop), t P1 -> t P2 ->
+    (forall z1 z2, P1 z1 -> P2 z2 -> P (z1 * z2)) -> t P.
+  
+  Fixpoint eval P (e : t P) {struct e} : {z : Z | P z}.
+    destruct e as [P z H | P1 P e1 Hcast | P1 P2 P e1 e2 Hcast | P1 P2 P e1 e2 Hcast].
+    - exists z; trivial.
+    
+    - destruct (eval _ e1) as (z1, H1).
+      exists (- z1); auto.
+    
+    - destruct (eval _ e1) as (z1, H1).
+      destruct (eval _ e2) as (z2, H2).
+      exists (z1 + z2); auto.
+    
+    - destruct (eval _ e1) as (z1, H1).
+      destruct (eval _ e2) as (z2, H2).
+      exists (z1 * z2); auto.
+  Defined.
+  
+  Module Test.
+    Definition example (x : Z) (H : x >= 10) : {y : Z | y >= 20}.
+      refine (
+        let y := x + 12 in
+        existT _ y _).
+      abstract (unfold y; omega).
+    Defined.
+    
+    Definition e (x : Z) (H : x >= 10) : t (fun y => y >= 20).
+      refine (
+        plus _ (const (fun x => x >= 10) x H) (const _ 12 eq_refl) _).
+      abstract (intros; omega).
+    Defined.
+    
+    Lemma ge15 : 15 >= 10.
+      omega.
+    Qed.
+    
+    Compute projT1 (eval (e ge15)).
+  End Test.
+End Arith.
 
 Module ArithAsm.
   Require Import ZArith.
   
   Local Open Scope Z_scope.
   
-  Inductive t : Set :=
-  | const (n : Z) | uminus | plus | minus | times.
-  
   Definition S := list Z.
   
-  Definition L (s : S) := unit.
-  
-  Definition lt (x y : nat * sigT L) : Prop :=
+  Definition lt (L : S -> Type) (x y : nat * sigT L) : Prop :=
     Peano.lt (fst x) (fst y).
   
-  Lemma lt_wf : well_founded lt.
-    apply well_founded_ltof.
+  Lemma lt_wf : forall L, well_founded (@lt L).
+    intro; apply well_founded_ltof.
   Defined.
   
-  Definition instr_of_state_update size (f : S -> S) : Instr.t lt_wf size.
+  Definition instr_of_state_update L size
+    (f : S -> S) (fl : forall s, L s -> L (f s))
+    : Instr.t (@lt_wf L) size.
     unfold Instr.t.
     refine (fun s ip =>
       existT _ (f s, ip) _).
     intros l Hip_valid.
     split; [now apply le_Sn_le |].
-    exists tt.
+    exists (fl s l).
     unfold lt; auto.
   Defined.
   
-  Definition instr_of_unop size (f : Z -> Z) : Instr.t lt_wf size :=
-    instr_of_state_update size (fun s =>
+  Definition instr_of_unop L size (f : Z -> Z) : Instr.t (@lt_wf L) size :=
+    instr_of_state_update L size (fun s =>
       match s with
       | n :: s => f n :: s
       | _ => s
@@ -177,6 +321,9 @@ Module ArithAsm.
       | n1 :: n2 :: s => f n1 n2 :: s
       | _ => s
       end).
+  
+  Inductive t (L : S -> Type) : Set :=
+  | const (n : Z) | uminus | plus | minus | times.
   
   Definition to_instr size (i : t) : Instr.t lt_wf size :=
     match i with
@@ -211,6 +358,10 @@ Module ArithAsm.
     Compute eval p3.
   End Test.
 End ArithAsm.
+
+
+
+
 
 
 
